clonemodel done

Impl/CloneModel.i.dfy
@@ -9,15 +9,10 @@ module CloneModel {
   import opened ViewOp
   import opened DiskOpModel
   import opened KeyType
-//   import opened Options
   import opened Sequences
   import opened Bounds
   import opened BucketsLib
   import opened BoundedPivotsLib
-
-  // import IT = IndirectionTable
-  // import opened NativeTypes
-  // import StateBCImpl
 
   lemma lemmaChildrenConditionsCloneNewRoot(s: BBC.Variables, oldroot: Node, from: Key, to: Key)
   requires s.Ready?
@@ -31,7 +26,7 @@ module CloneModel {
     BT.reveal_CutoffNodeAndKeepRight();
   }
 
-  function {:opaque} clone(s: BBC.Variables, from: Key, to: Key): (BBC.Variables)
+  function {:opaque} clone(s: BBC.Variables, from: Key, to: Key): (BBC.Variables, bool)
   requires BBC.Inv(s)
   requires s.Ready?
   requires BT.G.Root() in s.cache
@@ -40,7 +35,7 @@ module CloneModel {
       && s.frozenIndirectionTable.Some?
       && s.frozenIndirectionTable.value.hasEmptyLoc(BT.G.Root())
     ) then (
-      s
+      (s, false)
     ) else (
       var oldroot := s.cache[BT.G.Root()];
       lemmaChildrenConditionsOfNode(s, BT.G.Root());
@@ -55,15 +50,15 @@ module CloneModel {
             lemmaChildrenConditionsCloneNewRoot(s, oldroot, from, to);
             var s1 := writeBookkeeping(s, BT.G.Root(), newroot.children);
             var s' := s1.(cache := s1.cache[BT.G.Root() := newroot]);
-            s'
+            (s', true)
           ) else (
-            s
+            (s, false)
           )
         ) else (
-          s
+          (s, false)
         )
       ) else (
-        s
+        (s, false)
       )
     )
   }
@@ -71,15 +66,21 @@ module CloneModel {
   lemma cloneCorrect(s: BBC.Variables, from: Key, to: Key)
   requires clone.requires(s, from, to)
   requires s.totalCacheSize() <= MaxCacheSize()
-  ensures var s' := clone(s, from, to);
-    && s'.Ready?
-    && s'.totalCacheSize() <= MaxCacheSize()
-    && StateBCImpl.WFCache(s'.cache)
-    && betree_next(s, s')
+  ensures var (s', success) := clone(s, from, to);
+      && (success ==>
+        BBC.Next(s, s',
+          BlockDisk.NoDiskOp,
+          AdvanceOp(UI.CloneOp(BT.CloneMap(from, to)), true))
+      )
+      && (!success ==>
+        betree_next(s, s')
+      )
+      && (StateBCImpl.WFCache(s'.cache))
+      && s.totalCacheSize() == s'.totalCacheSize()
   {
     reveal_clone();
 
-    var s' := clone(s, from, to);
+    var (s', success) := clone(s, from, to);
     lemmaChildrenConditionsOfNode(s, BT.G.Root());
 
     if (
@@ -116,18 +117,13 @@ module CloneModel {
       writeCorrect(s, BT.G.Root(), newroot);
       assert s1 == s';
 
-
       var clone := BT.NodeClone(oldroot, newroot, from, to);
       var step := BT.BetreeClone(clone);
-      assert BT.ValidClone(clone);
 
+      assert BT.ValidClone(clone);
       BC.MakeTransaction1(s, s', BT.BetreeStepOps(step));
       assert BBC.BetreeMove(s, s', BlockDisk.NoDiskOp, AdvanceOp(UI.CloneOp(BT.CloneMap(from, to)), true), step);
       assert stepsBetree(s, s', AdvanceOp(UI.CloneOp(BT.CloneMap(from, to)), true), step);
-
-      // && betree_next(s, s')
-      assume false;
-
     } else {
       assert noop(s, s);
     }
